iodiv/TauIODiv.fst
@@ -80,7 +80,7 @@ let close (fd : file_descr) : IODiv unit (requires fun hist -> is_open fd hist) 
 let print (s:string) : IODiv unit (requires fun hist -> True) (ensures fun hist r -> terminates r /\ ret_trace r == [ EPrint s ]) =
   act_call Print s
 
-let iter #index #a #w (f : (j : index) -> IODIV (either index a) (w j)) (i : index) : IODIV a (i_iter w i) =
+let iter #index #a #w ($f : (j : index) -> IODIV (either index a) (w j)) (i : index) : IODIV a (i_iter w i) =
   IODIV?.reflect (dm_iter (fun j -> reify (f j)) i)
 
 let _repeat_with_inv_aux pre inv (body : iodiv_dm (either unit unit) (repeat_body_inv (fun _ -> pre) inv ())) :
